gw

random/landin.ml
@@ -1,0 +1,14 @@
+let backpatch =
+  let id x = x in
+  fun f ->
+    let x = ref id in
+    x:= (fun z -> f !x z);
+    !x
+
+let n = 10
+
+let _ =
+  let x = backpatch (fun r n -> if n = 0 then 1 else n * r (n-1)) 10 in
+  print_int x;
+  print_newline ()
+
