hashtbl/add_who.v
@@ -1,71 +1,94 @@
-(*whoSet*) Set Implicit Arguments. (*who*) 
-(*whoRequire*) Require Import WhoMap. (*who*) 
-(*whoVariable*) Variable ref : forall (a : Type) (k : key), Type. (*who*) 
-(*whoDefinition*) Definition ___get (A : Type) (k : key) (r : ref A k) (m : kmap) :=
-        __get A k m. (*who*) 
-(*whoNotation*) Notation "!!" := (___get) (at level 50). (*who*) 
+Set Implicit Arguments.
 
-(*whobeginsec*)
-Section sec. (*who*)
-  (*whobasiclogi*)  (*who*) (*whoarit*) Require Import WhoArith. (*who*) 
-  (*whocombine*) Definition combine: forall   (e1 e2 : kmap), kmap -> kmap ->
-                   kmap.  (*who*) Admitted.
-  (*whorestrict*) Definition restrict: forall   (e11 e21 : kmap), kmap ->
-                    kmap.  (*who*) Admitted.
-  (*whoArra*) Require Import WhoArray. (*who*) 
-  (*whoLis*) Require Import WhoList. (*who*) Admitted.Admitted.Admitted.
-  (*whoHashtb*) Require Import WhoHashtbl. (*who*) (*whoa*) Variables a :
-  Type. Variables r : key.  (*who*) 
-  (*whol*) Variable l: list ((hashkey) * a).  (*who*) 
-  (*whoh*) Variable h: ref (array (list ((hashkey) * a))) r.  (*who*) 
-  (*whokey*) Variable key: hashkey.  (*who*) 
-  (*whos*) Variable s: kmap.  (*who*) (*whoval*) Variable val: a.  (*who*) 
-  (*whoH*) Hypothesis H: 0 < (len (!! h s)).  (*who*) 
-  (*whoH1*) Hypothesis H1:
-            forall (i1:int),
-            (0 <= i1) ->
-            ((i1 < (len (!! h s))) ->
-             (forall (k1:hashkey),
-              forall (v1:a),
-              (l_in (k1 , v1) (get i1 (!! h s))) ->
-              ((mod (hash k1) (len (!! h s))) = i1))).  (*who*) 
-  (*whoH2*) Hypothesis H2: repr (!! h s) l.  (*who*) 
-  (*whos1*) Variable s1: kmap.  (*who*) 
-  (*whoH3*) Hypothesis H3: (!! h s) = (!! h s1).  (*who*) 
-  (*whos2*) Variable s2: kmap.  (*who*) 
-  (*whoH4*) Hypothesis H4: (!! h s1) = (!! h s2).  (*who*) 
-  (*whos3*) Variable s3: kmap.  (*who*) 
-  (*whoH5*) Hypothesis H5: (!! h s2) = (!! h s3).  (*who*) 
-  (*whos4*) Variable s4: kmap.  (*who*) 
-  (*whoH6*) Hypothesis H6:
-            (!! h s4) =
-            (set (mod (hash key) (len (!! h s1)))
-             (cons (key , val)
-              (get (mod (hash key) (len (!! h s1))) (!! h s2)))
-             (!! h s3)).  (*who*) 
-  (*whogoal*) Lemma goal: 0 < (len (!! h s4)). (*who*) 
-  Proof.  rewrite H6, <- update_length, <- H5, <- H4, <- H3. auto. Qed.
-  (*whobeginsec1*)
-  Section sec1. (*who*)
-    (*whoi*) Variable i: int.  (*who*) 
-    (*whoH7*) Hypothesis H7: 0 <= i.  (*who*) 
-    (*whoH8*) Hypothesis H8: i < (len (!! h s4)).  (*who*) 
-    (*whok*) Variable k: hashkey.  (*who*) (*whov*) Variable v: a.  (*who*) 
-    (*whoH9*) Hypothesis H9: l_in (k , v) (get i (!! h s4)).  (*who*) 
-    (*whogoal1*) Lemma goal1: (mod (hash k) (len (!! h s4))) = i. (*who*) 
-    Proof.
-      rewrite H6, H3, H4, H5 in *|-*; rewrite <- update_length in *|-*; clear H6 H5 H4 H3.
-      case_eq (Z_eq_dec i (mod (hash key) (length (!! h s3)))); intros; auto.
-      rewrite <- e, get_set_eq in H9; auto. 
-      generalize (in_inv H9); intros [K|K]. clear H0.
-      injection K; intros K1 K2; rewrite K1, K2 in *; clear K1 K2 K; auto.
-      apply H1 with v; auto.
-      rewrite get_set_neq in H9; auto.
-      apply H1 with v; auto. admit.
-    Qed.
-    (*whoendsec1*)
-    End sec1. (*who*)
-  (*whogoal2*) Lemma goal2: repr (!! h s4) (cons (key , val) l). (*who*) 
+
+
+Definition region : forall (u : Type) , Type. 
+  Proof.
+  Admitted.
+   
+Definition refty : forall (reg ty : Type) , Type. 
+  Proof.
+  Admitted.
+   
+Definition ref_get: forall (reg u : Type) ,  (region reg) -> (refty reg u) ->
+  u.
+  Proof.
+  Admitted.
+   
+Require Import WhoTuples.
+Require Import WhoArith.
+
+Require Import WhoMap.
+Require Import WhoArray.
+Require Import WhoList.
+
+Definition mmod:  Z -> Z -> Z.
+  Proof.
+  Admitted.
+   
+Hypothesis mmod1:
+  forall (a:Z), forall (b:Z), (0 <= (mmod a b)) /\ ((mmod a b) < b). 
+Definition hashkey : Type. 
+  Proof.
+  Admitted.
+   
+Definition hash:  hashkey -> Z.
+  Proof.
+  Admitted.
+   
+Definition repr: forall (a : Type) ,  (array (list (hashkey * a))) ->
+  (list (hashkey * a)) -> Prop.
+  Proof.
+  Admitted.
+   
+Section sec. 
+   Variables a r : Type.
   
-  (*whoendsec*)
-  End sec. (*who*)
+  Variable l:  list (hashkey * a). 
+  Variable h:  refty r (array (list (hashkey * a))). 
+  Variable key:  hashkey. 
+  Variable val:  a. 
+  Variable s:  region r. 
+  Hypothesis H:
+    0 <
+    ((@len  (list (hashkey * a)))
+     ((@ref_get  r (array (list (hashkey * a)))) s h)). 
+  Hypothesis H1:
+    forall (i:Z),
+    (0 <= i) ->
+    ((i <
+      ((@len  (list (hashkey * a)))
+       ((@ref_get  r (array (list (hashkey * a)))) s h)))
+     ->
+     (forall (k:hashkey),
+      forall (v:a),
+      ((@l_in  (hashkey * a)) ((@mk_2tuple  hashkey a) k v)
+       ((@get  (list (hashkey * a))) i
+        ((@ref_get  r (array (list (hashkey * a)))) s h)))
+      ->
+      (i =
+       (mmod (hash k)
+        ((@len  (list (hashkey * a)))
+         ((@ref_get  r (array (list (hashkey * a)))) s h)))))). 
+  Variable s1:  region r. 
+  Hypothesis H2:
+    ((@set  (list (hashkey * a)))
+     (mmod (hash key)
+      ((@len  (list (hashkey * a)))
+       ((@ref_get  r (array (list (hashkey * a)))) s h)))
+     ((@Cons  (hashkey * a)) ((@mk_2tuple  hashkey a) key val)
+      ((@get  (list (hashkey * a)))
+       (mmod (hash key)
+        ((@len  (list (hashkey * a)))
+         ((@ref_get  r (array (list (hashkey * a)))) s h)))
+       ((@ref_get  r (array (list (hashkey * a)))) s h)))
+     ((@ref_get  r (array (list (hashkey * a)))) s h))
+    = ((@ref_get  r (array (list (hashkey * a)))) s1 h). 
+  Lemma add_correct:
+    0 <
+    ((@len  (list (hashkey * a)))
+     ((@ref_get  r (array (list (hashkey * a)))) s1 h)). 
+    Proof.
+      rewrite <- H2. rewrite <- update_len; auto. apply mmod1.
+    Qed.
+     End sec.
