random/landin_who.v
@@ -1,0 +1,73 @@
+Set Implicit Arguments.
+
+
+
+Definition region : forall (u : Type) , Type. 
+  Proof.
+  Admitted.
+   
+Definition refty : forall (reg ty : Type) , Type. 
+  Proof.
+  Admitted.
+   
+Definition ref_get: forall (reg u : Type) ,  (region reg) -> (refty reg u) ->
+  u.
+  Proof.
+  Admitted.
+   
+Require Import WhoTuples.
+Require Import WhoArith.
+
+Require Import WhoMap.
+Require Import WhoArray.
+Require Import WhoList.
+
+Variables r : Type.
+
+Section sec. 
+   Variables a : Type.
+  
+  Variable p:  ((a -> (region r) -> Prop) * (a -> (region r) -> (region r) ->
+    a -> Prop)) -> (region r) -> Prop. 
+  Variable f_pre:  (refty r ((a -> (region r) -> Prop) * (a -> (region r) ->
+    (region r) -> a -> Prop))) -> unit -> Prop. 
+  Variable f_post:  (refty r ((a -> (region r) -> Prop) * (a -> (region r) ->
+    (region r) -> a -> Prop))) -> unit -> unit -> ((a -> (region r) ->
+    Prop) * (a -> (region r) -> (region r) -> a -> Prop)) -> Prop. 
+  Variable s:  region r. 
+  Hypothesis H:
+    forall (x:refty r ((a -> (region r) -> Prop) * (a -> (region r) ->
+    (region r) -> a -> Prop))),
+    (f_pre x tt) /\
+    (forall (anon_pre:a -> (region r) -> Prop),
+     forall (anon_post:a -> (region r) -> (region r) -> a -> Prop),
+     (f_post x tt tt
+      ((@mk_2tuple  (a -> (region r) -> Prop) (a -> (region r) ->
+       (region r) -> a -> Prop)) anon_pre anon_post))
+     ->
+     (forall (s1:region r),
+      (((@mk_2tuple  (a -> (region r) -> Prop) (a -> (region r) ->
+        (region r) -> a -> Prop)) anon_pre anon_post)
+       =
+       ((@ref_get  r ((a -> (region r) -> Prop) * (a -> (region r) ->
+        (region r) -> a -> Prop))) s1 x))
+      ->
+      (p
+       ((@mk_2tuple  (a -> (region r) -> Prop) (a -> (region r) ->
+        (region r) -> a -> Prop)) anon_pre anon_post)
+       s1))). 
+  Variable s1:  region r. 
+  Variable anon:  refty r ((a -> (region r) -> Prop) * (a -> (region r) ->
+    (region r) -> a -> Prop)). 
+  Hypothesis H1:
+    ((@mk_2tuple  (a -> (region r) -> Prop) (a -> (region r) -> (region r) ->
+     a -> Prop)) (fun (x:a) => (fun (cur:region r) => True))
+     (fun (x:a) =>
+     (fun (old:region r) => (fun (cur:region r) => (fun (anon1:a) => True)))))
+    =
+    ((@ref_get  r ((a -> (region r) -> Prop) * (a -> (region r) ->
+     (region r) -> a -> Prop))) s1 anon). 
+  Lemma backpatch_correct: f_pre anon tt. 
+    Proof.
+    Admitted.
+     End sec.
